Problem 1:
a. T(n)=2T(n-1)+1
   T(n-1)=2T(n-2)+2+1
   T(n-2)=2^2T(n-3)+4+2+1
   T(n-3)=2^3T(n-4)+8+2+1
   T(n)=2^k(n-k)+2^0+2^1+2^2+2^3+...+2^k-1
   k=n
   T(n)=2^n(n-n)+2^0+2^1+2^2+2^3+...+2^n-1
   T(n)=2^nT(0)+(n-1/i)∑2^i
   T(n)=2^n*1+2^n-1
   T(n)=2^(n+1)-1
b. T(n)=3T(n-1)+n
   T(n)=3^2T(n-1)+3n+n
   T(n)=3^3T(n-1)+9n+3n+n
   T(n)=3^k(n-k)+n(3^1+3^2+3+3^3+...+3^k-1)
   k=n
   T(n)=3^n(n-n)+n(3^1+3^2+3+3^3+...+3^n-1)
   T(n)=3^nT(0)+n((n-1/i)∑3^i)
   T(n)=3^n*1+n(3^n-1/2)
c. T(n)=9(n/2)+n^2
   T(n)=9(n/4)+(n/2)^2
   T(n)=9(n/8)+(n/4)^2
   T(n)=9^kT(n/2^k)+9^(k-1)(n/2^(k-1))^2
   T(n)=9^kT(n/2^k)+n^2((k-1/i)∑9^i(n/2^(k-1))^2)
   k=log(n)
   T(n)=9^log(n)T(n/2^log(n))+n^2((log(n)-1/i)∑9^i(n/2^(log(n)-1))^2)
   T(n)=9^log(n)*1+n^2((9^log(n)-1)/8-4(2^-2log(n)-1)/3)

   
